$p=mv$

- $p$ = momentum ($kgms^{-1}$)
- $m$ = mass (kg)
- $v$ = velocity ($ms^{-1}$)

$p_{before}=p_{after}$

- $p$ = momentum ($kgms^{-1}$)

$J=F(âˆ†t)=âˆ†p$

- $J$ = impulse (Ns)
- F = force (N)
- $t$ = time (s)
- $p$ = momentum ($kgms^{-1}$)

$a_UnderCurve=xy$

- $x$ = horizontal coordinate
- $y$ = vertical coordinate

$gradient={\frac{âˆ†y}{âˆ†x}}$

- $x$ = horizontal coordinate
- $y$ = vertical coordinate

---

$v_l=\frac{2Ï€r}T=\frac{âˆ†ğ›‰}{âˆ†t}=(\frac{2Ï€}T)r=Ï‰r$

- $v_l$ = linear speed ($ms^{-1}$)
- $r$ = radius ($m$)
- $T$ = time for a full rotation (s)

$Ï‰=\frac{2r}T=2rf=vr$

- $Ï‰$ = angular speed ($rad.sec^{-1}$)
- $r$ = radius ($m$)
- $T$ = time for a full rotation (s)
- $f$ = frequency (s$^{-1}$)
- $v$ = velocity ($ms^{-1}$)

$f=\frac1T$

- $f$ = frequency (hertz)
- $T$ = time for a full rotation (s)

$a_c=\frac{v^2}r=\frac{âˆ†w}{âˆ†t}=\frac{w_2-w_1}{t_2-t_1}=\frac{4Ï€^2r}{T^2}=v_{final}-v_{initial}$

- $a_c$ = angular acceleration ($rad.sec^-2$)
- $v$ = velocity ($ms^{-1}$)
- $r$ = radius ($m$)
- Ï‰ = angular speed ($rad.sec^{-1}$)
- $t$ = time (s)
- $T$ = time for a full rotation (s)

$a=\frac{âˆ†v}{âˆ†t}$

- $a$ = acceleration ($ms^{-2}$)
- $v$ = velocity ($ms^{-1}$)
- $t$ = time ($s$)

$F=ma=\frac{mv^2}r=mÏ‰^2r$

- F = force (N)
- m = mass (kg)
- $a$ = acceleration ($ms^{-2}$)
- v = velocity (ms$^{-1}$)
- $r$ = radius ($m$)
- Ï‰ = angular speed ($rad.sec^{-1}$)

$F_c=\frac{mcdot v^2}r$

- $F_c$ = Centripetal force (N)
- $m$ = mass (kg)
- $v$ = velocity ($ms^{-1}$)
- $r$ = radius ($m$)

---

$W=Fs=Fscosğ›‰=âˆ†E_k$

- $W$ = work done ($J$)
- F = applied force ($N$)
- s = displacement ($m$)
- ğ›‰ = angle between force and displacement (Ëš)
- $E_k$ = kinetic energy (J)

$E_k=\frac12mv^2$

- $E_k$ = kinetic energy (J)
- $m$ = mass (kg)
- v = velocity (ms$^{-1}$)

$E_p=mgh_{(gravitational)}=\frac12kâˆ†x^2_{(spring)}$

- $E_p$ = gravitational energy (J)
- $m$ = mass (kg)
- $g$ = gravity (10 $ms^{-2}$)
- $h$ = height ($m$)
- $k$ = spring constant ($Nm^{-1}$)
- $x$ = extension (m)

$E_t=E_k+E_p$

- $E_t$ = mechanical energy (J)
- $E_k$ = kinetic energy (J)
- $E_p$ = gravitational energy (J)

$P=Fv=\frac Et=\frac Wt$

- $P$ = power (W)
- F = force (N)
- $v$ = velocity ($ms^{-1}$)
- $E$ = energy (J)
- $t$ = time (s)
- $W$ = work (J)

%% Whatever the **** this is %%
Â¡â„¢Â£Â¢âˆÂ§Â¶â€¢ÂªÂºâ€“â‰ Å“âˆ‘Â´Â®â€ Â¥Â¨Ë†Ã¸Ï€â€œâ€˜Â«Ã¥ÃŸâˆ‚Æ’Â©Ë™âˆ†ËšÂ¬â€¦Ã¦Î©â‰ˆÃ§âˆšâˆ«ËœÂµâ‰¤â‰¥Ã·â„â‚¬â€¹â€ºï¬ï¬‚â€¡Â°Â·â€šâ€”Â±Å’â€Â´â€°Ë‡ÃÂ¨Ë†Ã˜âˆâ€â€™Â»Ã…ÃÃÃËÃ“Ã”ï£¿Ã’ÃšÃ†Â¸Ë›Ã‡â—ŠÄ±ËœÃ‚Â¯Ë˜Â¿
